src/program_proof/tulip/program/replica/replica_apply_commit.v
@@ -141,7 +141,8 @@ Section program.
         symmetry in Hcpmabs.
         pose proof (lookup_kmap_eq_Some _ _ _ _ _ _ Hcpmabs Hm) as (ts' & Hts' & Hcpmts).
         assert (ts' = ts) as -> by word.
-        by rewrite /execute_cmds foldl_snoc /= execute_cmds_unfold Hexec /= Hterm Hcpmts.
+        rewrite /execute_cmds foldl_snoc /= execute_cmds_unfold Hexec /= Hterm Hcpmts.
+        by case_decide.
       }
     }
     iDestruct (big_sepM2_dom with "Hprepm") as %Hdomprepm.
@@ -166,7 +167,8 @@ Section program.
       pose proof (lookup_kmap_eq_None _ _ _ _ _  Hcpmabs Hnone) as Hcpmnone.
       specialize (Hcpmnone ts).
       unshelve epose proof (Hcpmnone _) as Hcpmts; first word.
-      by rewrite /execute_cmds foldl_snoc /= execute_cmds_unfold Hexec /= Hterm Hcpmts.
+      rewrite /execute_cmds foldl_snoc /= execute_cmds_unfold Hexec /= Hterm Hcpmts.
+      by case_decide.
     }
   Qed.
 
